\documentclass{article}
\usepackage{color}
\usepackage{bigints}
\usepackage[italicdiff]{physics}
\color{white}
\definecolor{Red}{RGB}{124,10,2}
\begin{document}
\pagecolor{Red}
\title{Solution to Calculus with Calvin\textsc{\char13}s Problem}
\author{Jose Bedoya}
\maketitle
\section{Question}
{\LARGE
$$I=\bigintss_{0}^{1} \frac{\ln \left(x+1\right)\ln x}{x}\,dx$$
}
\section{Solution}
{\Large
Knowing,
$$\ln \left(x+1\right)=\sum_{n=1}^{\infty} \left(-1\right)^{n-1}\frac{x^n}{n}$$

\vspace{3mm}
We have
$$I=\sum_{n=1}^{\infty}\frac{\left(-1\right)^{n-1}}{n}\bigintsss_{0}^{1}x^{n-1}\ln x\,dx$$

\vspace{3mm}
Applying IBP, we get
$$I=\sum_{n=1}^{\infty}\frac{\left(-1\right)^{n-1}}{n}\left(\frac{x^n\ln x}{n}\Big|_0^1-\frac{1}{n}\bigintsss_{0}^{1}x^{n-1}\,dx\right)$$
$$=\sum_{n=1}^{\infty}\frac{\left(-1\right)^n}{n^3}$$

\vspace{4mm}
Let\textsc{\char13}s try to find a closed expression for this sum. We know:
$$\zeta\left(3\right)=\sum_{n=1}^{\infty}\frac{1}{n^3}$$

\vspace{3mm}
As you can see, our sum is equal to the even inverse cubes minus the odd ones. So, let\textsc{\char13}s find an expression for the odd ones
$$\sum_{n=1}^{\infty}\frac{1}{\left(2n+1\right)^3}=\sum_{n=1}^{\infty}\left(\frac{1}{n^3}-\frac{1}{\left(2n\right)^3}\right)$$
$$=\frac{7\zeta\left(3\right)}{8}$$

\vspace{3mm}
Therefore,
$$\sum_{n=1}^{\infty}\frac{\left(-1\right)^n}{n^3}=\sum_{n=1}^{\infty}\left(\frac{1}{\left(2n\right)^3}-\frac{1}{\left(2n+1\right)^3}\right)$$

\vspace{5mm}
Thus,
}
{\LARGE
$$I=\frac{-3\zeta\left(3\right)}{4}$$
}
\end{document}