\documentclass{article}
\usepackage{color}
\usepackage{bigints}
\usepackage[italicdiff]{physics}
\color{white}
\definecolor{Blue}{RGB}{0,33,71}
\begin{document}
\pagecolor{Blue}
\title{Solution to Mathemaddict\textsc{\char13}s Problem}
\author{Jose Bedoya}
\maketitle
\section{Question}
{\LARGE
$$I=\bigintss_{1}^{\infty} \frac{2x\{x\}-\{x\}^2}{x^2\lfloor x\rfloor^2}\,dx=\frac{\pi^A}{B}-\phi^C$$

\vspace{4mm}
Then,
$$L=\lim_{\theta\to C} \frac{\sin\left(A\theta\right)\sec \left(\theta\right)}{B\theta}=\,?$$

\vspace{3mm}
Note: $\{x\}=x-\lfloor x\rfloor$
}
\section{Solution}
{\Large
Let\textsc{\char13}s expand the integral using the definition of the fractional part
$$I=\bigintsss_{1}^{\infty}\frac{2x^2-2x\lfloor x\rfloor-x^2+2x\lfloor x\rfloor-\lfloor x\rfloor^2}{x^2\lfloor x\rfloor^2}\,d $$

\vspace{5mm}
Simplifying and by the definition of the floor function 
$$I=\sum_{k=1}^{\infty}\bigintsss_{k}^{k+1}\frac{1}{k^2}-\frac{1}{x^2}\,dx$$

\vspace{4mm}
Therefore,
\newpage
$$I=\sum_{k=1}^{\infty}\left(\frac{x}{k^2}\Big|_k^{k+1}+\frac{1}{x}\Big|_k^{k+1}\right)$$
$$=\sum_{k=1}^{\infty}\left(\frac{1}{k^2}+\frac{1}{k+1}-\frac{1}{k}\right)$$

\vspace{3mm}
Evaluating the series we get
$$I=\frac{\pi^2}{6}-1$$

\vspace{3mm}
Clearly,
$$A=2,\,B=6,\, C=1$$

\vspace{5mm}
Substituting in the limit, we get
$$\lim_{\theta\to0} \frac{\sin\left(2\theta\right)\sec\left(\theta\right)}{6\theta}=\frac{1}{3}$$

\vspace{3mm}
Our final answer is
}
{\LARGE
$$L=\frac{1}{3}$$
}
\end{document} 