\documentclass{article}
\usepackage[utf8]{inputenc}
\usepackage{amsmath}
\usepackage{amssymb}

\title{Calculus With Calvin QD. 27}
\author{Shreenabh Agrawal}
\date{\today}

\begin{document}

\maketitle

\section{Question}
Compute the Integral:
$$I=\int\limits_{0}^{1} \frac{\ln (1+x) \ln (x)}{x} \: d x$$

\section{Solution}
We know the Series Expansion:
$$\ln (1+x)=\sum_{n=1}^{\infty} \frac{(-1)^{n-1} x^{n}}{n}$$
$$\Rightarrow I=\int\limits_{0}^{1} \sum_{n=1}^{\infty} \frac{(-1)^{n-1} x^{n-1}}{n} \: \ln (x) \: d x$$

$$\therefore I=\sum_{n=1}^{\infty} \frac{(-1)^{n-1}}{n} \int\limits_{0}^{1} x^{n-1} \ln (x) \: d x$$

We know the Formula,
$$I_{(m, n)}=\int\limits_{0}^{1} x^{m} \ln ^{n}(x) \: d x=(-1)^{n} \frac{n !}{(m+1)^{n+1}}$$

[This can be derived using IBP and Recursion] \\

Comparing $I_{(m, n)}$ with $I$, we have,
$$m = n-1$$
$$n = 1$$

$$\therefore I_{(n-1,1)}=\frac{(-1)}{n^{2}}$$

$$\begin{array}{l}
\begin{aligned}
\Rightarrow \quad I &=\sum_{n=1}^{\infty} \frac{(-1)^{n-1}}{n} \times \frac{(-1)}{n^{2}} \\
&=\sum_{n=1}^{\infty} \frac{(-1)^{n}}{n^{3}}
\end{aligned}
\end{array}$$

Expanding this, we have:

$$\begin{aligned}
I&=-\frac{1}{1^{3}}+\frac{1}{2^{3}}-\frac{1}{3^{3}}+\frac{1}{4^{3}}-\ldots \\
&=-\frac{1}{1^{3}}-\frac{1}{2^{3}}-\frac{1}{3^{3}}-\frac{1}{4^{3}}-\ldots 
{+2\left[\frac{1}{2^{3}}+\frac{1}{4^{3}}+\ldots\right]}\\
&=-\zeta(3)+\left(\frac{1}{2^{3} \cdot 1^{3}}+\frac{1}{2^{3} \cdot 2^{3}}+\frac{1}{2^{3} \cdot 3^{3}}+\ldots\right) \\
&=-\zeta(3)+\frac{1}{4} \zeta(3) \\
\end{aligned}$$

Thus, the final answer is:
$$\boxed{I=-\frac{3 \: \zeta(3)}{4}}$$

\end{document}
