\documentclass{article}
\usepackage[utf8]{inputenc}
\usepackage[dvipsnames]{xcolor}
\usepackage{amsmath}
\title{}

\begin{document}
\maketitle
\pagecolor{black}
\textcolor{white}{
\begin{center}
    An Interesting Summation\\ 
    \smallskip{}
    {\tiny Without Complex Analysis!}
    $$\sum_{n=-\infty}^{\infty} \frac{1}{n^2+a^2} = \frac{\pi \coth(a \pi)}{a}$$
    Swipe For EZ Derivation \textcolor{red}{$\Rightarrow$}
\end{center}
\newpage
First we factor the expression in the denominator as 
$$\frac{1}{n^2+a^2} = \frac{1}{(n+ai)(n-ai)} = \frac{1}{2ai}\left( \frac{1}{n-ai} - \frac{1}{n+ai}\right)$$
$$ \sum_{n=1}^{\infty} \frac{1}{n^2+a^2} = \frac{1}{2ai} \left( \sum_{n=1}^{\infty} \frac{1}{n-ai} - \frac{1}{n+ai} \right) $$
We can evaluate the inner summation by considering $\psi(1+ai)$ and $\psi(1-ai)$
\begin{equation}
    \psi(1+ai) = -\gamma + \sum_{n=1}^{\infty} \frac{1}{n} - \frac{1}{n+ai} 
\end{equation}
\begin{equation}
    \psi(1-ai) = -\gamma + \sum_{n=1}^{\infty} \frac{1}{n} - \frac{1}{n-ai}
\end{equation}
Doing (2) $-$ (1) gives us 
$$ \psi(1+ai) - \psi(1-ai) = \sum_{n=1}^{\infty} \frac{1}{n-ai} - \frac{1}{n+ai}$$
Using the functional equation (derived last post)
$$ \psi(1+ai) = \psi(ai) + \frac{1}{ai} $$
$$ \sum_{n=1}^{\infty} \frac{1}{n-ai} - \frac{1}{n+ai} = \frac{1}{ai} + \psi(ai) - \psi(1-ai) $$
\newpage
$$ \sum_{n=1}^{\infty} \frac{1}{n-ai} - \frac{1}{n+ai} = \frac{1}{ai} + \psi(ai) - \psi(1-ai) $$
Using the reflection formula (derived last post), we would then have 
$$ \sum_{n=1}^{\infty} \frac{1}{n-ai} - \frac{1}{n+ai} = \frac{1}{ai} - \pi \cot(a\pi i)$$
Note the negative sign being there because the original reflection formula says $$\psi(1-x) - \psi(x) = \pi \cot(\pi x)$$
Going back to the original sum, we get 
$$ \sum_{n=1}^{\infty} \frac{1}{n^2+a^2} = \frac{1}{2ai} \left( \sum_{n=1}^{\infty} \frac{1}{n-ai} - \frac{1}{n+ai} \right) = \frac{1}{2ai} \left( \frac{1}{ai} - \pi \cot(a\pi i) \right)$$
Recalling $\coth(x) = i\cot(ix)$
$$ \sum_{n=1}^{\infty} \frac{1}{n^2+a^2} = \frac{1}{2ai} \left( \frac{1}{ai} - \frac{\pi \coth(a\pi)}{i} \right) = -\frac{1}{2a^2}+ \frac{\pi \coth(a\pi)}{2a}$$
$$ \sum_{n=-\infty}^{\infty} \frac{1}{n^2+a^2} = \frac{1}{a^2} + 2 \sum_{n=1}^{\infty} \frac{1}{n^2+a^2} = \frac{1}{a^2} + 2\left( -\frac{1}{2a^2}+ \frac{\pi \coth(a\pi)}{2a} \right) $$
$$ \sum_{n=-\infty}^{\infty} \frac{1}{n^2+a^2} = \frac{\pi \coth(a \pi)}{a} $$
\newpage
    $$\sum_{n=-\infty}^{\infty} \frac{1}{n^2+a^2} = \frac{\pi \coth(a \pi)}{a}$$
    \begin{center}
       \large{For more, Follow}
    \end{center}
}
\end{document}
